factor out backtranslation function

FullAbstractionFE.v
@@ -17,25 +17,7 @@ Require Import LogRelFE.LemmasLR.
 Require Import BacktransFE.Emulate.
 Require Import BacktransFE.InjectExtract.
 Require Import BacktransFE.UpgradeDowngrade.
-
-Definition backtranslateCtx n τ Cu : F.PCtx := (F.eraseAnnot_pctx (F.pctxA_cat
-                      (F.a_papp₂ τ (UValFE n (compfe_ty τ)) (injectA n τ) F.a_phole)
-                      (emulate_pctx n Cu))).
-
-Lemma backtranslateCtx_works {Cu m n d p τs τu ts tu} :
-  ValidTy τu →
-  dir_world_prec m n d p →
-  ⟪ ea⊢ Cu : E.empty, compfe_ty τs → E.empty, τu ⟫ →
-  ⟪ pempty ⊩ ts ⟦ d, n ⟧ tu : embed τs ⟫ →
-  ⟪ pempty ⊩ (F.pctx_app ts (backtranslateCtx m τs Cu)) ⟦ d, n ⟧ E.pctx_app tu (eraseAnnot_pctx
-      Cu) : pEmulDV m p τu ⟫.
-Proof.
-  intros vτu dwp tCu lr; destruct p; unfold backtranslateCtx;
-  rewrite F.eraseAnnot_pctx_cat, F.pctx_cat_app;
-  [change pempty with (toEmulDV m precise E.empty) | change pempty with (toEmulDV m imprecise E.empty)];
-  eapply emulate_pctx_works; eauto using dwp_precise, dwp_imprecise with tyvalid;
-  eapply inject_works_open; eauto using dwp_precise, dwp_imprecise with tyvalid.
-Qed.
+Require Import BacktransFE.Backtrans.
 
 Lemma equivalencePreservation {t₁ t₂ τ} :
   ⟪ F.empty ⊢ t₁ : τ ⟫ →
