BacktransFI/Backtrans.v
@@ -1,0 +1,29 @@
+Require Import StlcIso.SpecAnnot.
+Require Import CompilerFI.Compiler.
+
+Require Import UValFI.UVal.
+
+Require Import LogRelFI.LR.
+
+Require Import BacktransFI.Emulate.
+Require Import BacktransFI.InjectExtract.
+Require Import BacktransFI.UpgradeDowngrade.
+
+Definition backtranslateCtx n τ Cu : F.PCtx := (F.eraseAnnot_pctx (F.pctxA_cat
+                      (F.a_papp₂ τ (UValFI n (compfi_ty τ)) (injectA n τ) F.a_phole)
+                      (emulate_pctx n Cu))).
+
+Lemma backtranslateCtx_works {Cu m n d p τs τu ts tu} :
+  ValidTy τu →
+  dir_world_prec m n d p →
+  ⟪ ia⊢ Cu : I.empty, compfi_ty τs → I.empty, τu ⟫ →
+  ⟪ pempty ⊩ ts ⟦ d, n ⟧ tu : embed τs ⟫ →
+  ⟪ pempty ⊩ (F.pctx_app ts (backtranslateCtx m τs Cu)) ⟦ d, n ⟧ I.pctx_app tu (eraseAnnot_pctx
+      Cu) : pEmulDV m p τu ⟫.
+Proof.
+  intros vτu dwp tCu lr; destruct p; unfold backtranslateCtx;
+  rewrite F.eraseAnnot_pctx_cat, F.pctx_cat_app;
+  [change pempty with (toEmulDV m precise I.empty) | change pempty with (toEmulDV m imprecise I.empty)];
+  eapply emulate_pctx_works; eauto using dwp_precise, dwp_imprecise with tyvalid;
+  eapply inject_works_open; eauto using dwp_precise, dwp_imprecise with tyvalid.
+Qed.
