BacktransIE/Backtrans.v
@@ -1,0 +1,28 @@
+Require Import StlcEqui.SpecAnnot.
+Require Import CompilerIE.Compiler.
+
+Require Import UValIE.UVal.
+
+Require Import LogRelIE.LR.
+
+Require Import BacktransIE.Emulate.
+Require Import BacktransIE.InjectExtract.
+Require Import BacktransIE.UpgradeDowngrade.
+
+Definition backtranslateCtx n τ Cu : I.PCtx := (I.eraseAnnot_pctx (I.pctxA_cat
+                      (I.ia_papp₂ τ (UValIE n τ) (injectA n τ) I.ia_phole)
+                      (emulate_pctx n Cu))).
+
+Lemma backtranslateCtx_works {Cu m n d p τs τu ts tu} :
+  ValidTy τu → ValidTy τs →
+  dir_world_prec m n d p →
+  ⟪ ea⊢ Cu : empty, τs → empty, τu ⟫ →
+  ⟪ pempty ⊩ ts ⟦ d, n ⟧ tu : embed τs ⟫ →
+  ⟪ pempty ⊩ (I.pctx_app ts (backtranslateCtx m τs Cu)) ⟦ d, n ⟧ E.pctx_app tu (eraseAnnot_pctx
+      Cu) : pEmulDV m p τu ⟫.
+  intros vτu vτs dwp tCu lr; destruct p; unfold backtranslateCtx;
+  rewrite I.eraseAnnot_pctx_cat, I.pctx_cat_app;
+  [change pempty with (toEmulDV m precise empty) | change pempty with (toEmulDV m imprecise I.empty)];
+  eapply emulate_pctx_works; eauto using dwp_precise, dwp_imprecise with tyvalid;
+  eapply inject_works_open; eauto using dwp_precise, dwp_imprecise with tyvalid.
+Qed.
